12UnstructuredMemory/Unstructuring.thy
@@ -3,34 +3,34 @@ theory Unstructuring
 begin
 
 fun restructure :: "unstr_state \<Rightarrow> flat_state" where
-  "restructure (US h hp x p e ep vs vp sh sp 0) = 
+  "restructure (US h hp e ep vs vp sh sp 0) = 
     FS (H h hp) (H e ep) (listify' vs vp) []"
-| "restructure (US h hp x p e ep vs vp sh sp (Suc pc)) = 
+| "restructure (US h hp e ep vs vp sh sp (Suc pc)) = 
     FS (H h hp) (H e ep) (listify' vs vp) (Suc pc # listify' sh sp)"
 
 theorem completeu [simp]: "cd \<tturnstile> \<Sigma>\<^sub>u \<leadsto>\<^sub>u \<Sigma>\<^sub>u' \<Longrightarrow> iter (\<tturnstile> cd \<leadsto>\<^sub>f) (restructure \<Sigma>\<^sub>u) (restructure \<Sigma>\<^sub>u')"
 proof (induction \<Sigma>\<^sub>u \<Sigma>\<^sub>u' rule: evalu.induct)
-  case (evu_lookup_zero cd pc x h hp p e ep vs vp sh sp)
+  case (evu_lookup cd pc x h sh sp y hp e ep vs vp)
   then show ?case by simp
 next
-  case (evu_pushcon cd pc k h hp x p e ep vs vp sh sp)
+  case (evu_pushcon cd pc k h hp e ep vs vp sh sp)
   then show ?case by simp
 next
-  case (evu_pushlam cd pc pc' h hp x p e ep vs vp sh sp)
+  case (evu_pushlam cd pc pc' h hp e ep vs vp sh sp)
   then show ?case by simp
 next
-  case (evu_apply cd pc h vs vp hp x p e ep sh sp)
+  case (evu_apply cd pc h vs vp hp e ep sh sp)
   then show ?case by simp
 next
-  case (evu_return cd pc h hp x p e ep vs vp sh sp)
+  case (evu_return cd pc h hp e ep vs vp sh sp)
   then show ?case by simp
 next
-  case (evu_jump cd pc h vs vp hp x p e ep sh sp)
+  case (evu_jump cd pc h vs vp hp e ep sh sp)
   then show ?case by simp
-qed simp_all
+qed
 
-lemma [dest]: "FS h env vs sfs = restructure \<Sigma> \<Longrightarrow> \<exists>h' hp x p e ep vs' vp sh sp pc. 
-  \<Sigma> = US h' hp x p e ep vs' vp sh sp pc \<and> h = H h' hp \<and> env = H e ep \<and> vs = listify' vs' vp \<and> 
+lemma [dest]: "FS h env vs sfs = restructure \<Sigma> \<Longrightarrow> \<exists>h' hp e ep vs' vp sh sp pc. 
+  \<Sigma> = US h' hp e ep vs' vp sh sp pc \<and> h = H h' hp \<and> env = H e ep \<and> vs = listify' vs' vp \<and> 
     ((pc = 0 \<and> sfs = []) \<or> (\<exists>pc'. pc = Suc pc' \<and> sfs = pc # listify' sh sp))"
   by (induction \<Sigma> rule: restructure.induct) simp_all
 
@@ -39,8 +39,8 @@ theorem correctu [simp]: "cd \<tturnstile> restructure \<Sigma>\<^sub>u \<leadst
 proof (induction "restructure \<Sigma>\<^sub>u" \<Sigma>\<^sub>f' rule: evalf.induct)
   case (evf_lookup cd pc x env p v h vs sfs)
   hence "FS h env vs (Suc pc # p # sfs) = restructure \<Sigma>\<^sub>u" by simp
-  then obtain h' hp xx pp e ep vs' vp sh sp where S: "
-    \<Sigma>\<^sub>u = US h' hp xx pp e ep vs' vp sh sp (Suc pc) \<and> h = H h' hp \<and> env = H e ep \<and> 
+  then obtain h' hp e ep vs' vp sh sp where S: "
+    \<Sigma>\<^sub>u = US h' hp e ep vs' vp sh sp (Suc pc) \<and> h = H h' hp \<and> env = H e ep \<and> 
       vs = listify' vs' vp \<and> p # sfs = listify' sh sp" by fastforce
 
 
@@ -49,7 +49,7 @@ proof (induction "restructure \<Sigma>\<^sub>u" \<Sigma>\<^sub>f' rule: evalf.in
 
 
 
-  have "iter (\<tturnstile> cd \<leadsto>\<^sub>u) (US h' hp xx pp e ep vs' vp sh sp (Suc pc)) \<Sigma>\<^sub>u' \<and> FS h env (v # vs) (pc # p # sfs) = restructure \<Sigma>\<^sub>u'" by simp
+  have "iter (\<tturnstile> cd \<leadsto>\<^sub>u) (US h' hp e ep vs' vp sh sp (Suc pc)) \<Sigma>\<^sub>u' \<and> FS h env (v # vs) (pc # p # sfs) = restructure \<Sigma>\<^sub>u'" by simp
   with S show ?case by blast
 next
   case (evf_pushcon cd pc k h h' v env vs p sfs)
