13AssemblyCode/Assemble.thy
@@ -1,0 +1,128 @@
+theory Assemble
+  imports AssemblyCode "../12UnstructuredMemory/UnstructuredMemory"
+begin  
+
+primrec assemble' :: "(nat \<Rightarrow> nat) \<Rightarrow> byte_code \<Rightarrow> assm list" where
+  "assemble' mp (BLookup x) = [
+      AMov ACC SP,
+      ASub ACC 1,
+      ALod ACC Stk ACC,
+      ALdI ACC2 x,
+      AAdd ACC2 1,
+      AJIZ ACC2 4,
+      ASub ACC2 1,
+      AAssert ACC ((>) 1),
+      ASub ACC 1,
+      ALod ACC Hp ACC,
+      AJmp 5,
+      AAssert ACC ((>) 1),
+      ASub ACC 2,
+      ALod ACC Hp ACC,
+      ASto Val VP ACC,
+      AAdd VP 1]"
+| "assemble' mp (BPushCon k) = [
+      ASto Val VP HP, 
+      AAdd VP 1, 
+      ALdI ACC 0, 
+      ASto Hp HP ACC, 
+      AAdd HP 1, 
+      ALdI ACC k, 
+      ASto Hp HP ACC, 
+      AAdd HP 1, 
+      ALdI ACC 0, 
+      ASto Hp HP ACC, 
+      AAdd HP 1]"
+| "assemble' mp (BPushLam pc) = [
+      ASto Val VP HP, 
+      AAdd VP 1, 
+      ALdI ACC 1, 
+      ASto Hp HP ACC, 
+      AAdd HP 1, 
+      AMov ACC SP, 
+      ASub ACC 1,
+      ALod ACC Stk ACC,
+      ASto Hp HP ACC, 
+      AAdd HP 1, 
+      ALdI ACC (mp pc), 
+      ASto Hp HP ACC, 
+      AAdd HP 1]"
+| "assemble' mp BApply = [
+      ASub VP 1,
+      ALod ACC Val VP,
+      ASto Env EP ACC,
+      AAdd EP 1,
+      ASub VP 1,
+      ALod ACC Val VP,
+      ALod ACC2 Hp ACC,
+      ASub ACC2 1,
+      AAssert ACC2 ((=) 0),
+      AAdd ACC 1,
+      ALod ACC2 Hp ACC,
+      ASto Env EP ACC2,
+      AAdd EP 1,
+      ASto Stk SP EP,
+      AAdd SP 1,
+      AAdd ACC 1,
+      ALod ACC Hp ACC,
+      ASto Stk SP ACC,
+      AAdd SP 1]"
+| "assemble' mp BReturn = [
+      ASub SP 1, 
+      ALod ACC Stk SP, 
+      AIJp ACC]"
+| "assemble' mp BJump = [
+      ASub VP 1,
+      ALod ACC Val VP,
+      ASto Env EP ACC,
+      AAdd EP 1,
+      ASub VP 1,
+      ALod ACC Val VP,
+      ALod ACC2 Hp ACC,
+      ASub ACC2 1,
+      AAssert ACC2 ((=) 0),
+      AAdd ACC 1,
+      ALod ACC2 Hp ACC,
+      ASto Env EP ACC2,
+      AAdd EP 1,
+      ASub SP 1,
+      AAdd ACC 1,
+      ALod ACC Hp ACC,
+      ASto Stk SP ACC,
+      ASub SP 1,
+      ASto Stk SP EP,
+      AAdd SP 2]"
+
+primrec assemble :: "byte_code list \<Rightarrow> assm list \<times> (nat \<Rightarrow> nat)" where
+  "assemble [] = ([], id)"
+| "assemble (op # cd) = (
+    let (cd', mp) = assemble cd
+    in let op' = assemble' mp op
+    in (op' @ cd', \<lambda>x. if x < length cd then mp x else mp x + length op'))"
+
+primrec assemble_state :: "(nat \<Rightarrow> nat) \<Rightarrow> unstr_state \<Rightarrow> assm_state" where
+  "assemble_state mv (US h hp e ep vs vp sh sp pc) = AS (\<lambda>r. case r of
+      HP \<Rightarrow> hp 
+    | EP \<Rightarrow> ep
+    | VP \<Rightarrow> vp
+    | SP \<Rightarrow> sp
+    | ACC \<Rightarrow> undefined) (\<lambda>m. case m of
+      Hp \<Rightarrow> h
+    | Env \<Rightarrow> e
+    | Val \<Rightarrow> vs
+    | Stk \<Rightarrow> sh) pc"
+
+theorem completea [simp]: "cd\<^sub>a \<tturnstile> \<Sigma>\<^sub>a \<leadsto>\<^sub>a \<Sigma>\<^sub>a' \<Longrightarrow> 
+  \<exists>cd\<^sub>b mp \<Sigma>\<^sub>u \<Sigma>\<^sub>u'. assemble cd\<^sub>b = (cd\<^sub>a, mp) \<and> assemble_state mp \<Sigma>\<^sub>u = \<Sigma>\<^sub>a \<and> 
+    assemble_state mp \<Sigma>\<^sub>u' = \<Sigma>\<^sub>a' \<and> iter (\<tturnstile> cd\<^sub>b \<leadsto>\<^sub>u) \<Sigma>\<^sub>u \<Sigma>\<^sub>u'"
+  by (induction cd\<^sub>a \<Sigma>\<^sub>a \<Sigma>\<^sub>a' rule: evala.induct) blast
+
+theorem correcta [simp]: "cd\<^sub>b \<tturnstile> \<Sigma>\<^sub>u \<leadsto>\<^sub>u \<Sigma>\<^sub>u' \<Longrightarrow> assemble cd\<^sub>b = (cd\<^sub>a, mp) \<Longrightarrow>
+    iter (\<tturnstile> cd\<^sub>a \<leadsto>\<^sub>a) (assemble_state mp \<Sigma>\<^sub>u) (assemble_state mp \<Sigma>\<^sub>u')"
+  by (induction cd\<^sub>b \<Sigma>\<^sub>u \<Sigma>\<^sub>u' rule: evalu.induct) blast
+
+theorem correcta_iter [simp]: "iter (\<tturnstile> cd\<^sub>b \<leadsto>\<^sub>u) \<Sigma>\<^sub>u \<Sigma>\<^sub>u' \<Longrightarrow> assemble cd\<^sub>b = (cd\<^sub>a, mp) \<Longrightarrow>
+    iter (\<tturnstile> cd\<^sub>a \<leadsto>\<^sub>a) (assemble_state mp \<Sigma>\<^sub>u) (assemble_state mp \<Sigma>\<^sub>u')"
+  by (induction \<Sigma>\<^sub>u \<Sigma>\<^sub>u' rule: iter.induct)
+     (force, metis correcta iter_append)
+
+end
