13AssemblyCode/AssemblyCode.thy
@@ -1,0 +1,88 @@
+theory AssemblyCode
+  imports Main
+begin
+
+datatype memory = Hp | Env | Val | Stk
+
+datatype register = HP | EP | VP | SP | ACC | ACC2
+
+datatype assm = 
+    ALdI register nat
+  | ALod register memory register
+  | ASto memory register register
+  | AMov register register
+  | AAdd register nat
+  | ASub register nat
+  | AIJp register (* indirect jump *)
+  | AJIZ register nat (* forwards jump *)
+  | AJmp nat (* backwards jump *)
+  | AAssert register "nat \<Rightarrow> bool"
+
+datatype assm_state = AS "register \<Rightarrow> nat" "memory \<Rightarrow> nat \<Rightarrow> nat" nat
+
+inductive evala :: "assm list \<Rightarrow> assm_state \<Rightarrow> assm_state \<Rightarrow> bool" (infix "\<tturnstile> _ \<leadsto>\<^sub>a" 50) where 
+  eva_ldi [simp]: "cd ! pc = ALdI r k \<Longrightarrow> cd \<tturnstile> AS rs mem (Suc pc) \<leadsto>\<^sub>a AS (rs(r := k)) mem pc"
+| eva_lod [simp]: "cd ! pc = ALod r m ptr \<Longrightarrow> 
+    cd \<tturnstile> AS rs mem (Suc pc) \<leadsto>\<^sub>a AS (rs(r := mem m (rs ptr))) mem pc"
+| eva_sto [simp]: "cd ! pc = ASto m ptr r \<Longrightarrow> 
+    cd \<tturnstile> AS rs mem (Suc pc) \<leadsto>\<^sub>a AS rs (mem(m := (mem m)(rs ptr := rs r))) pc"
+| eva_mov [simp]: "cd ! pc = AMov r1 r2 \<Longrightarrow> cd \<tturnstile> AS rs mem (Suc pc) \<leadsto>\<^sub>a AS (rs(r1 := rs r2)) mem pc"
+| eva_add [simp]: "cd ! pc = AAdd r k \<Longrightarrow> cd \<tturnstile> AS rs mem (Suc pc) \<leadsto>\<^sub>a AS (rs(r := rs r + k)) mem pc"
+| eva_sub [simp]: "cd ! pc = ASub r k \<Longrightarrow> cd \<tturnstile> AS rs mem (Suc pc) \<leadsto>\<^sub>a AS (rs(r := rs r - k)) mem pc"
+| eva_ijp [simp]: "cd ! pc = AIJp r \<Longrightarrow> cd \<tturnstile> AS rs mem (Suc pc) \<leadsto>\<^sub>a AS rs mem (rs r)"
+| eva_jiz_z [simp]: "cd ! pc = AJIZ r k \<Longrightarrow> rs r = 0 \<Longrightarrow>
+    cd \<tturnstile> AS rs mem (Suc pc) \<leadsto>\<^sub>a AS rs mem (pc - k)"
+| eva_jiz_s [simp]: "cd ! pc = AJIZ r pc' \<Longrightarrow> rs r = Suc y \<Longrightarrow>
+    cd \<tturnstile> AS rs mem (Suc pc) \<leadsto>\<^sub>a AS rs mem pc"
+| eva_jmp [simp]: "cd ! pc = AJmp k \<Longrightarrow> cd \<tturnstile> AS rs mem (Suc pc) \<leadsto>\<^sub>a AS rs mem (pc + k)"
+| eva_assert [simp]: "cd ! pc = AAssert r p \<Longrightarrow> p (rs r) \<Longrightarrow> 
+    cd \<tturnstile> AS rs mem (Suc pc) \<leadsto>\<^sub>a AS rs mem pc"
+
+theorem determinisma: "cd \<tturnstile> \<Sigma> \<leadsto>\<^sub>a \<Sigma>' \<Longrightarrow> cd \<tturnstile> \<Sigma> \<leadsto>\<^sub>a \<Sigma>'' \<Longrightarrow> \<Sigma>' = \<Sigma>''"
+proof (induction cd \<Sigma> \<Sigma>' rule: evala.induct)
+  case (eva_ldi cd pc r k rs mem)
+  from eva_ldi(2, 1) show ?case 
+    by (induction cd "AS rs mem (Suc pc)" \<Sigma>'' rule: evala.induct) simp_all
+next
+  case (eva_lod cd pc r m ptr rs mem)
+  from eva_lod(2, 1) show ?case 
+    by (induction cd "AS rs mem (Suc pc)" \<Sigma>'' rule: evala.induct) simp_all
+next
+  case (eva_sto cd pc m ptr r rs mem)
+  from eva_sto(2, 1) show ?case 
+    by (induction cd "AS rs mem (Suc pc)" \<Sigma>'' rule: evala.induct) simp_all
+next
+  case (eva_mov cd pc r1 r2 rs mem)
+  from eva_mov(2, 1) show ?case 
+    by (induction cd "AS rs mem (Suc pc)" \<Sigma>'' rule: evala.induct) simp_all
+next
+  case (eva_add cd pc r k rs mem)
+  from eva_add(2, 1) show ?case 
+    by (induction cd "AS rs mem (Suc pc)" \<Sigma>'' rule: evala.induct) simp_all
+next
+  case (eva_sub cd pc r k rs mem)
+  from eva_sub(2, 1) show ?case 
+    by (induction cd "AS rs mem (Suc pc)" \<Sigma>'' rule: evala.induct) simp_all
+next
+  case (eva_ijp cd pc r rs mem)
+  from eva_ijp(2, 1) show ?case 
+    by (induction cd "AS rs mem (Suc pc)" \<Sigma>'' rule: evala.induct) simp_all
+next
+  case (eva_jiz_z cd pc r pc' rs mem)
+  from eva_jiz_z(3, 1, 2) show ?case 
+    by (induction cd "AS rs mem (Suc pc)" \<Sigma>'' rule: evala.induct) simp_all
+next
+  case (eva_jiz_s cd pc r pc' rs y mem)
+  from eva_jiz_s(3, 1, 2) show ?case 
+    by (induction cd "AS rs mem (Suc pc)" \<Sigma>'' rule: evala.induct) simp_all
+next
+  case (eva_jmp cd pc k rs mem)
+  from eva_jmp(2, 1) show ?case 
+    by (induction cd "AS rs mem (Suc pc)" \<Sigma>'' rule: evala.induct) simp_all
+next
+  case (eva_assert cd pc r p rs mem)
+  from eva_assert(3, 1, 2) show ?case 
+    by (induction cd "AS rs mem (Suc pc)" \<Sigma>'' rule: evala.induct) simp_all
+qed
+
+end
